src/deletion.lean
@@ -1,6 +1,7 @@
 import basic
 import rotations
 import tactic.linarith
+import tactic.induction
 set_option pp.generalized_field_notation false
 
 universe u
@@ -17,16 +18,6 @@ variables {α : Type u}
 --   simp [delRoot, shrink, delRoot_core],
 -- end
 
-lemma delRoot_some (l r sh : btree α) (x k : nat) (v a : α) (h : shrink l = some (x, a, sh)) :
-  delRoot (btree.node l k v r) = 
-    if height r > height sh + 1 then rotL (btree.node sh x a r) 
-    else btree.node sh x a r :=
-begin
-  simp [delRoot], 
-  rw h,
-  refl,
-end
-
 lemma delRoot_ordered (t : btree α) :
   ordered t → ordered (delRoot t) :=
 begin
@@ -36,21 +27,16 @@ begin
     simp [delRoot, ordered],
   },
   case node: tl tk ta tr ihl ihr {
-    cases tl,
-    case empty {
-      simp [delRoot, shrink, delRoot_core],
-      simp [ordered] at h₁,
-      apply and.left h₁,
+    cases' delRoot_delRoot_view (node tl tk ta tr),
+    case nonempty_empty {
+      sorry
     },
-    case node : tll tlk tla tlr {
-      simp [delRoot, shrink, delRoot_core],
-      rcases (shrink_core (shrink tlr) tll tlk tla tlr) with ⟨x, a, sh⟩,
-      simp [delRoot_core],
-      by_cases c₁ : (height sh + 1 < height tr),
-      { simp [if_pos c₁],
-        sorry,
-      },
-      { sorry },
+    case nonempty_nonempty₁ {
+      rw h_2; clear h_2,
+      sorry,
+    },
+    case nonempty_nonempty₂ {
+      sorry
     }
   }
 end
@@ -68,14 +54,14 @@ begin
     simp [delete],
     simp [ordered] at h₁,
     by_cases c₁ : (k = tk),
-    { simp [if_pos c₁], 
+    { simp [if_pos c₁],
       apply delRoot_ordered,
       rw ordered,
       assumption,
     },
     { simp [if_neg c₁],
       by_cases c₂ : (k < tk),
-      { simp [if_pos c₂], 
+      { simp [if_pos c₂],
         by_cases c₃ : (height (delete k tl) + 1 < height tr),
         { simp only [if_pos c₃],
           sorry,
@@ -96,19 +82,19 @@ begin
       },
       { simp [if_neg c₂],
         by_cases c₃ : (height (delete k tr) + 1 < height tl),
-        { simp [if_pos c₃], 
+        { simp [if_pos c₃],
           sorry,
         },
-        { simp [if_neg c₃, ordered], 
+        { simp [if_neg c₃, ordered],
           split,
           { apply and.left h₁, },
           { split,
             { apply ihr,
-              apply and.left (and.right h₁), 
+              apply and.left (and.right h₁),
             },
             { split,
               { apply and.left (and.right (and.right h₁)), },
-              { sorry, }, 
+              { sorry, },
             },
           },
         },
